[STRINGS] Add HEXCHARS=>UBYTE8S and HEXSTRING=>UBYTE8S.
These are inverses of the existing UBYTE8S=>HEXCHARS and UBYTE8S=>HEXSTRING.

books/kestrel/utilities/strings/hexchars.lisp
@@ -92,3 +92,50 @@
        :rule-classes :linear
        :enable str::natchars16
        :prep-books ((include-book "std/lists/len" :dir :system))))))
+
+;;;;;;;;;;;;;;;;;;;;;;;;;;;;;;;;;;;;;;;;;;;;;;;;;;;;;;;;;;;;;;;;;;;;;;;;;;;;;;;;
+
+(define hexchars=>ubyte8s ((chars (and (str::hex-digit-listp chars)
+                                       (true-listp chars)
+                                       (evenp (len chars)))))
+  :returns (bytes (unsigned-byte-listp 8 bytes))
+  :parents (8bitbytes-hexchars-conversions)
+  :short "Convert an even-length sequence of hexadecimal digit characters
+          to a list of natural numbers below 256."
+  :long
+  (xdoc::topp
+   "Each pair of hexadecimal digit characters is turned into sa number.
+    Each such two-digit hexadecimal notation is treated as big endian,
+    i.e. the most significant digit appears first.")
+  (mbe :logic (cond ((endp chars) nil)
+                    (t (b* ((hi-digit (str::hex-digit-val (car chars)))
+                            (lo-digit (str::hex-digit-val (cadr chars)))
+                            (byte (+ (* hi-digit 16) lo-digit))
+                            (bytes (hexchars=>ubyte8s (cddr chars))))
+                         (cons byte bytes))))
+       :exec (hexchars=>ubyte8s-aux chars nil))
+
+  :prepwork
+  ((define hexchars=>ubyte8s-aux ((chars (and (str::hex-digit-listp chars)
+                                              (true-listp chars)
+                                              (evenp (len chars))))
+                                  (rev-bytes (unsigned-byte-listp 8 rev-bytes)))
+     (cond ((endp chars) (rev rev-bytes))
+           (t (b* ((hi-digit (str::hex-digit-val (car chars)))
+                   (lo-digit (str::hex-digit-val (cadr chars)))
+                   (byte (+ (* hi-digit 16) lo-digit)))
+                (hexchars=>ubyte8s-aux (cddr chars) (cons byte rev-bytes)))))
+     :enabled t))
+
+  :verify-guards nil ; done below
+
+  ///
+
+  (defrulel verify-guards-lemma
+    (implies (and (str::hex-digit-listp chars)
+                  (true-listp chars)
+                  (evenp (len chars)))
+             (equal (hexchars=>ubyte8s-aux chars rev-bytes)
+                    (revappend rev-bytes (hexchars=>ubyte8s chars)))))
+
+  (verify-guards hexchars=>ubyte8s))
